Add documentation for foos 1, 2, 3, 4, 5, 7, 8, 9, 16, 19, 20, and give them descriptive names.
Refactor Dns into DnsSchema, Dns (containing spec, honing, and spec-dependent lemmas), and DnsLemmas (containing definitions and refinement lemmas).

src/Examples/DnsServer/Dns.v
@@ -6,149 +6,14 @@ Require Import Coq.Vectors.Vector
 
 Require Import Fiat.QueryStructure.Automation.AutoDB
         Fiat.QueryStructure.Implementation.DataStructures.BagADT.BagADT
-        Fiat.Examples.DnsServer.packet
         Fiat.QueryStructure.Automation.IndexSelection
         Fiat.QueryStructure.Specification.SearchTerms.ListPrefix
         Fiat.QueryStructure.Automation.SearchTerms.FindSuffixSearchTerms
-        Fiat.QueryStructure.Automation.QSImplementation.
-Open Scope list.
+        Fiat.QueryStructure.Automation.QSImplementation
+        Fiat.Examples.DnsServer.packet
+        Fiat.Examples.DnsServer.DnsSchema
+        Fiat.Examples.DnsServer.DnsLemmas.
 
-Definition upperbound {A} (f : A -> nat) (rs : list A) (r : A) :=
-  forall r', List.In r' rs -> f r >= f r'.
-
-Section FueledFix.
-  (* TODO: Find a home for these more definitions in the Common folder. *)
-
-  Variable A : Type. (* Argument Type *)
-  Variable R : Type. (* Return Type *)
-
-  Fixpoint FueledFix (fuel : nat) (base : Comp R)
-                     (body : (A -> Comp R) -> A -> Comp R) (arg : A)
-  : Comp R :=
-    match fuel with
-      | O => base
-      | S fuel' => body (FueledFix fuel' base body) arg
-    end.
-End FueledFix.
-
-(* Can rewrite under Fueled Fix at the moment,
-as the condition on the body is not a proper relation. :p *)
-(* TODO: figure out a definition for pointwise_refine that is a
-   proper (i.e. reflexive and transitive) relation.
- *)
-(*
-Print respectful.
-
-Definition pointwise_refine {A R}
-  (f g : (A -> Comp R) -> A -> Comp R) :=
-  forall (rec rec' : A -> Comp R) (a : A),
-    pointwise_relation A (@refine R) rec rec'
-    -> refine (f rec a) (g rec' a).
-
-Lemma reflexive_pR {A R : Type} :
-  forall A R, Reflexive (@pointwise_refine A R).
-Proof.
-  unfold Reflexive, pointwise_refine, pointwise_relation.
-  intros.
-  (* Doesn't work if x is (fun rec a => {r | ~ rec ~> r} :p *)
-Admitted.
-
-Lemma transitive_pR {A R : Type} :
-  forall A R, Transitive (@pointwise_refine A R).
-Proof.
-  unfold Transitive, pointwise_refine, pointwise_relation; intros.
-  etransitivity.
-  apply H; eauto.
-  apply H0. reflexivity.
-Qed.
-
-Add Parametric Morphism A R i
-: (@FueledFix A R i)
-    with signature
-    ((@refine R)
-       ==> (@pointwise_refine A R)
-      ==> (@eq A)
-      ==> (@refine R))
-      as refineFix.
-Proof.
-  simpl; induction i; intros; simpl.
-  - assumption.
-  - unfold pointwise_refine, pointwise_relation, Proper, respectful in *.
-    eapply H0.
-    intros.
-    generalize (IHi _ _ H _ _ H0 a); eauto.
-Qed.
-*)
-
-(* TODO: Agree on a notation for our fueled fix function. *)
-Notation "'Repeat' fuel 'initializing' a 'with' arg 'defaulting' rec 'with' base {{ bod }} " :=
-  (FueledFix fuel base (fun rec a => bod) arg)
-    (no associativity, at level 50,
-     format "'Repeat' '[hv'  fuel  '/' 'initializing'  a  'with'  arg '/'  'defaulting'  rec  'with'  base  '/' {{ bod  }} ']' ").
-
-Section FueledFixRefinements.
-  (* TODO: Find a home for these refinements in the Computation folder. *)
-
-  Variable A : Type. (* Argument Type *)
-  Variable R : Type. (* Return Type *)
-
-  (* TODO Lemmas for refining FueledFix. *)
-
-  Lemma refine_FueledFix_Bind (B : Type) :
-    forall fuel body (base : Comp R) (arg : A) (k k' : R -> Comp B),
-      refine (r <- base; k r) (r <- base; k' r)
-      -> (forall fuel',
-            refine (a <- FueledFix fuel' base body arg; k a)
-                   (a <- FueledFix fuel' base body arg; k' a)
-            -> refine
-                 (a <- FueledFix (S fuel') base body arg; k a)
-                 (a <- FueledFix (S fuel') base body arg; k' a))
-      ->  refine (a <- FueledFix fuel base body arg; k a)
-                 (a <- FueledFix fuel base body arg; k' a).
-  Proof.
-    induction fuel; eauto.
-  Qed.
-
-End FueledFixRefinements.
-
-Section FilteredList.
-
-  Definition filtered_list {A}
-             (xs : list A)
-             (P : Ensemble A)
-    := fold_right (fun (a : A) (l : Comp (list A)) =>
-                     l' <- l;
-                     b <- { b | decides b (P a) };
-                     if b
-                     then ret (a :: l')
-                     else ret l'
-                  ) (ret nil) xs.
-
-End FilteredList.
-
-(* Agree on this notation. *)
-Notation "'unique' b , P ->> s 'otherwise' ->> s'" :=
-  (b' <- {b' | forall b, b' = Some b <-> P};
-   If_Opt_Then_Else b' (fun b => s) s') (at level 70).
-
-Definition is_empty {A} (l : list A) :=
-  match l with nil => true | _ => false end.
-
-Definition get_name (r : DNSRRecord) : list string := r!sNAME.
-Definition name_length (r : DNSRRecord) := List.length (get_name r).
-
-Notation "[[ x 'in' xs | P ]]" := (filtered_list xs (fun x => P)) (at level 70) : comp_scope.
-
-Definition DnsSchema :=
-  Query Structure Schema
-        [ relation sCOLLECTIONS has
-                   schema <sNAME :: name,
-          sTYPE :: RRecordType,
-          sCLASS :: RRecordClass,
-          sTTL :: nat,
-          sDATA :: string>
-          where (fun t t' => t!sNAME = t'!sNAME -> t!sTYPE <> CNAME) ]
-        enforcing [ ].
 
 Definition DnsSig : ADTSig :=
   ADTsignature {
@@ -156,6 +21,7 @@ Definition DnsSig : ADTSig :=
       Method "AddData" : rep x DNSRRecord -> rep x bool,
       Method "Process" : rep x packet -> rep x packet
     }.
+
 Definition DnsSpec : ADT DnsSig :=
   QueryADTRep DnsSchema {
     Def Constructor "Init" (_ : unit) : rep := empty,
@@ -167,93 +33,42 @@ Definition DnsSpec : ADT DnsSig :=
       let t := qtype (questions p) in
       Repeat 1 initializing n with qname (questions p)
                defaulting rec with (ret (buildempty p))
-
          {{ rs <- For (r in sCOLLECTIONS)      (* Bind a list of all the DNS entries *)
                   Where (IsPrefix n r!sNAME) (* prefixed with [n] to [rs] *)
+                  (* prefix: "com.google" is a prefix of "com.google.scholar" *)
                   Return r;
             If (is_empty rs)        (* Are there any matching records? *)
-            Then
+            Then                    (* TODO: reverse these if/then cases *)
               bfrs <- [[r in rs | upperbound name_length rs r]]; (* Find the best match (largest prefix) in [rs] *)
               b <- { b | decides b (forall r, List.In r bfrs -> n = r!sNAME) };
               if b                (* If the record's QNAME is an exact match  *)
               then
-                unique b,
+                unique b,                         (* only one match (unique / otherwise) *)
                 List.In b bfrs /\ b!sTYPE = CNAME     (* If the record is a CNAME, *)
                                /\ t <> CNAME ->>      (* and the query did not request a CNAME *)
 
                   p' <- rec b!sNAME;                  (* Recursively find records matching the CNAME *)
                                                     (* ?? Shouldn't this use the sDATA ?? *)
                   ret (addan p' b)
+                      (* addan : packet -> DNSRRecord -> packet *)
                 otherwise ->>     (* Copy the records into the answer section of an empty response *)
+                (* multiple matches -- add them all as answers in the packet *)
                   ret (List.fold_left addan bfrs (buildempty p))
-              else
+              else              (* prefix but record's QNAME not an exact match *)
+                (* return all the prefix records that are nameserver records -- 
+                 ask the authoritative servers *)
                 bfrs' <- [[x in bfrs | x!sTYPE = NS]];
                 ret (List.fold_left addns bfrs' (buildempty p))
             Else ret (buildempty p) (* No matching records! *)
           }}}.
-(* Parade of admitted refinement lemmas. Should go in a DNS Refinements file. *)
 
-Lemma foo1 :
-  forall (n : DNSRRecord) (R : @IndexedEnsemble DNSRRecord),
-    n!sTYPE <> CNAME
-    -> refine {b |
-               decides b
-                       (forall tup' : IndexedTuple,
-                          R tup' ->
-                          n!sNAME = (indexedElement tup')!sNAME -> n!sTYPE <> CNAME)}
-              (ret true).
-Proof.
-  intros; refine pick val true; [ reflexivity | simpl; intros; assumption ].
-Qed.
+(* -------------------------------------------------------------------------------------- *)
 
-Lemma foo2 :
-  forall (n : DNSRRecord) (R : @IndexedEnsemble DNSRRecord),
-    n!sTYPE = CNAME
-    -> refine {b |
-               decides b
-                       (forall tup' : IndexedTuple,
-                          R tup' ->
-                          n!sNAME = (indexedElement tup')!sNAME -> n!sTYPE <> CNAME)}
-              (b <- {b |
-                     decides b
-                             (exists tup' : IndexedTuple,
-                                R tup' /\
-                                n!sNAME = (indexedElement tup')!sNAME)};
-               ret (negb b)).
-Proof.
-   repeat match goal with
-    | _ : _ ↝ _ |- _ => computes_to_inv
-    | _ : negb ?v = _ |- _ => destruct v; simpl in *; subst
-    | _ : ex _ |- _ => destruct_ex
-    | _ => progress first [ intro | computes_to_econstructor | simpl; intuition; eauto ]
-          end.
-Qed.
+(* Refinement lemmas that depend on DnsSchema (other lemmas are in DnsLemmas) *)
 
-Lemma foo4 :
-  forall (n : DNSRRecord) (R : @IndexedEnsemble DNSRRecord),
-    refine {b |
-            decides b
-                    (forall tup' : IndexedTuple,
-                       R tup' ->
-                       (indexedElement tup')!sNAME = n!sNAME
-                       -> (indexedElement tup')!sTYPE <> CNAME)}
-           (b <- {b |
-                  decides b
-                          (exists tup' : IndexedTuple,
-                             R tup' /\
-                             n!sNAME = (indexedElement tup')!sNAME
-                             /\ (indexedElement tup')!sTYPE = CNAME)};
-            ret (negb b)).
-Proof.
-  repeat match goal with
-    | _ : _ ↝ _ |- _ => computes_to_inv
-    | _ : negb ?v = _ |- _ => destruct v; simpl in *; subst
-    | _ : ex _ |- _ => destruct_ex
-    | _ => progress first [ intro | computes_to_econstructor | simpl; intuition; eauto ]
-         end.
-Qed.
-
-Lemma foo3 :
+(* implement the DNS record constraint check as code that counts the number of occurrences of
+the constraint being broken (refines the boolean x1 in AddData) *)
+Lemma refine_count_constraint_broken :
   forall (n : DNSRRecord) (r : UnConstrQueryStructure DnsSchema),
     refine {b |
             decides b
@@ -269,7 +84,7 @@ Lemma foo3 :
             ret (beq_nat count 0) Else ret true).
 Proof.
   intros; setoid_rewrite refine_pick_decides at 1;
-  [ | apply foo2 | apply foo1 ].
+  [ | apply refine_is_CNAME__forall_to_exists | apply refine_not_CNAME__independent ].
   (* refine existence check into query. *)
   match goal with
       |- context[{b | decides b
@@ -302,23 +117,26 @@ Proof.
 Qed.
 
 
-Lemma foo5 :
+(* uses refine_forall_to_exists; refines x2 in AddData 
+very similar to refine_count_constraint_broken; comments below are relative to refine_count_constraint_broken *)
+Lemma refine_count_constraint_broken' :
   forall (n : DNSRRecord) (r : UnConstrQueryStructure DnsSchema),
     refine {b |
             decides b
                     (forall tup' : @IndexedTuple (GetHeading DnsSchema sCOLLECTIONS),
                        (r!sCOLLECTIONS)%QueryImpl tup' ->
-                       (indexedElement tup')!sNAME = n!sNAME
-                       -> (indexedElement tup')!sTYPE <> CNAME)}
+                       (indexedElement tup')!sNAME = n!sNAME (* switched *)
+                       -> (indexedElement tup')!sTYPE <> CNAME)} (* indexedElement tup', not n *)
+           (* missing the If/Then statement *)
            (count <- Count
                   For (UnConstrQuery_In r ``(sCOLLECTIONS)
                                         (fun tup : Tuple =>
                                            Where (n!sNAME = tup!sNAME
-                                                  /\ tup!sTYPE = CNAME )
+                                                  /\ tup!sTYPE = CNAME ) (* extra /\ condition *)
                                                  Return tup ));
             ret (beq_nat count 0)).
 Proof.
-  intros; setoid_rewrite foo4.
+  intros; setoid_rewrite refine_forall_to_exists.
   (*refine existence check into query. *)
   match goal with
       |- context[{b | decides b
@@ -347,486 +165,64 @@ Proof.
   setoid_rewrite negb_involutive; f_equiv.
 Qed.
 
-Lemma foo7 {heading}
-: forall (R : Ensemble (@IndexedTuple heading))
-         (P : Ensemble Tuple) (P_dec : DecideableEnsemble P)
-         (l : list Tuple),
-    For (QueryResultComp
-           R
-           (fun tup => Where (P tup)
-                             (Return tup))) ↝ l  ->
-    forall (P' : Ensemble Tuple) (P'_dec : DecideableEnsemble P'),
-      refine (For (QueryResultComp
-                     R
-                     (fun tup => Where (P tup /\ P' tup)
-                                       (Return tup))))
-             (ret (filter DecideableEnsembles.dec l)).
-Proof.
-  Local Transparent Query_For.
-  unfold Query_For, QueryResultComp, Query_Return;
-    intros; computes_to_inv.
-  refine pick val _; eauto.
-  simplify with monad laws.
-  unfold refine; intros; computes_to_inv; computes_to_econstructor.
-  instantiate (1 := (filter (@dec _ _ P'_dec) v)).
-  - clear H0 H H' v1; generalize dependent v; induction v0.
-    + simpl; intros; computes_to_inv; subst; reflexivity.
-    + simpl; intros; computes_to_inv; subst; apply IHv0 in H'0'; clear IHv0.
-      destruct (@dec _ P' P'_dec a) eqn: dec_a; unfold Query_Where in *; destruct H'0.
-      * pose proof dec_a as dec_a'; apply dec_decides_P in dec_a.
-        repeat computes_to_inv; repeat computes_to_econstructor.
-        intuition eauto. eauto.
-        apply eq_ret_compute; destruct (@dec _ P P_dec a) eqn: dec__a.
-        apply dec_decides_P in dec__a; apply H in dec__a;
-        computes_to_inv; subst; simpl; rewrite dec_a'; reflexivity.
-        apply Decides_false in dec__a; apply H0 in dec__a; subst; reflexivity.
-      * pose proof dec_a as dec_a'; apply Decides_false in dec_a.
-        repeat computes_to_inv; repeat computes_to_econstructor.
-        intuition eauto. eauto.
-        apply eq_ret_compute; destruct (@dec _ P P_dec a) eqn: dec__a.
-        apply dec_decides_P in dec__a; apply H in dec__a;
-        computes_to_inv; subst; simpl; rewrite dec_a'; reflexivity.
-        apply Decides_false in dec__a; apply H0 in dec__a; subst; reflexivity.
-  - refine pick val _; auto; subst.
-    apply filter_permutation_morphism; [ reflexivity | assumption ].
-Qed.
+(* -------------------------------------------------------------------------------------- *)
 
-Lemma foo8 {A}
-: forall (c c' : bool) (t e e' : A),
-    (c = true -> c' = true)
-    -> (if c then (if c' then t else e) else e') = if c then t else e'.
-Proof.
-  intros; destruct c; destruct c'; try reflexivity.
-  assert (true = true); [ reflexivity | apply H in H0; discriminate ].
-Qed.
+(* TODO: working on this code; please excuse the comments *)
 
-Lemma foo9 {A}
-: forall (l : list A) (pred : A -> bool),
-    beq_nat (Datatypes.length l) 0 = true
-    ->  beq_nat (Datatypes.length (filter pred l)) 0 = true.
-Proof.
-  induction l; intros; simpl; try inversion H.
-  reflexivity.
-Qed.
-
-Lemma andb_implication_preserve :
-  forall a b, (a = true -> b = true) -> a = b && a.
-Proof.
-  intros; destruct a; destruct b; symmetry; auto.
-Qed.
-Lemma andb_permute :
-  forall a b c, a && (b && c) = b && (a && c).
-  intros.
-  repeat rewrite andb_assoc.
-  replace (a && b) with (b && a) by apply andb_comm.
-  reflexivity.
-Qed.
-
-(*Ltac PrefixSearchTermFinderEqSolve :=
-  intros; unfold PrefixSearchTermMatcher; simpl;
-   apply andb_implication_preserve; find_if_inside; intros;
-   match goal with
-     | H : _ = _ |- _ =>
-       setoid_rewrite H;
-         erewrite prefixBool_reflexive; reflexivity
-     | _ => erewrite prefixBool_reflexive; reflexivity
-     | _ => discriminate
-   end.
-Ltac PrefixSearchTermNormalizer idx :=
-  generalize dependent idx;
-  let a' := fresh in
-  let ha := fresh in
-  match goal with
-    | |- forall a, _ = PrefixSearchTermMatcher ?st (@?h a) =>
-      intros a'; remember (h a') as ha; generalize ha
-  end.
-Ltac PrefixSearchTermFinder' idx :=
-  PrefixSearchTermNormalizer idx;
-  match goal with
-    (* case prefix match *)
-    | |- forall a, prefixBool ?n a!sNAME && @?f a = PrefixSearchTermMatcher ?st a =>
-      instantiate (1 := {| pst_name := n; pst_filter := f |}); reflexivity
-    (* case equality *)
-    | |- forall a, ?[list_eq_dec string_dec ?n a!sNAME] && @?f a =
-                   PrefixSearchTermMatcher ?st a =>
-      instantiate
-        (1 := {| pst_name := n;
-                 pst_filter := fun a => ?[list_eq_dec string_dec n a!sNAME] && f a |});
-        PrefixSearchTermFinderEqSolve
-    | |- forall a, ?[list_eq_dec string_dec a!sNAME ?n] && @?f a =
-                   PrefixSearchTermMatcher ?st a =>
-      instantiate
-        (1 := {| pst_name := n;
-                 pst_filter := fun a => ?[list_eq_dec string_dec a!sNAME n] && f a |});
-        PrefixSearchTermFinderEqSolve
-  end.
-Ltac AdjustAndRec terminal term :=
-  let aterm := fresh in
-  first [
-      (* if we get the exact match, we're done !*)
-      assert (aterm : terminal = term) by reflexivity; clear aterm |
-      match term with
-        | ?left && ?right =>
-          first [
-              (* if the left term is the exact match, also done! *)
-              assert (aterm : left = terminal) by reflexivity; clear aterm |
-              (* if the right term is the exact match, just need to switch! *)
-              assert (aterm : right = terminal) by reflexivity; clear aterm;
-                replace (left && right) with
-                (right && left) by apply andb_comm |
-              (* now try recursively on the left term *)
-              (AdjustAndRec terminal left);
-                match goal with
-                  | |- context [ (terminal && ?rem) && right ] =>
-                    replace ((terminal && rem) && right) with
-                    (terminal && (rem && right)) by apply andb_assoc
-                end |
-              (* and now the righ term *)
-              (AdjustAndRec terminal right);
-                match goal with
-                  | |- context [ left && (terminal && ?rem) ] =>
-                    replace (left && (terminal && rem)) with
-                    (terminal && (left && rem)) by apply andb_permute
-                end ]
-      end ].
-Ltac AdjustAnd terminal ensure_and :=
-  match goal with
-    | |- ?filter = _ => AdjustAndRec terminal filter
-  end;
-  match ensure_and with
-    | true =>
-      match goal with
-        | |- _ && _ = _ => idtac
-        | |- ?x = _ => rewrite <- (andb_true_r x)
-      end
-    | false => idtac
-  end.
-Ltac PrefixSearchTermFinder :=
-  let idx := fresh in
-  intros idx;
-  match goal with
-    | |- context [ prefixBool ?n ?n' ] =>
-      AdjustAnd (prefixBool n n') true; PrefixSearchTermFinder' idx
-    (* ensure_and can be false, but need some more thought *)
-    | |- context [ ?[list_eq_dec string_dec ?n ?n'] ] =>
-      AdjustAnd (?[list_eq_dec string_dec n n']) true; PrefixSearchTermFinder' idx
-    | |- _ => PrefixSearchTermNormalizer idx;
-        match goal with
-          (* catch all case; ignore search term, use only the filter *)
-          (* only when wildcard is idtac, when this tactic gets used *)
-          | |- forall a, @?f a = PrefixSearchTermMatcher ?st a =>
-            instantiate (1 := {| pst_name := nil; pst_filter := f |}); reflexivity
-        end
-  end.
-
-Lemma foo10
-: forall (n : DNSRRecord) (b c d e : bool), exists st, forall (a : DNSRRecord * nat),
-    ?[list_eq_dec string_dec (fst a)!sNAME n!sNAME] =
-    PrefixSearchTermMatcher st (fst a).
-Proof.
-  eexists.
-  PrefixSearchTermFinder.
-Qed.
-Print foo10.
-Lemma foo10' : forall n : DNSRRecord, forall b c d, exists st, forall (a : DNSRRecord * nat),
-    b && ( c && d ) && (?[list_eq_dec string_dec (fst a)!sNAME n!sNAME]) && (?[RRecordType_dec (fst a)!sTYPE CNAME]) =
-    PrefixSearchTermMatcher st (fst a).
-Proof.
-  eexists; PrefixSearchTermFinder.
-Qed.
-Print foo10'.
-Lemma foo13
-: forall n : DNSRRecord, exists st, forall a : DNSRRecord,
-    prefixBool (n!sNAME) (a!sNAME)  =
-    PrefixSearchTermMatcher st a.
-Proof.
-  eexists; PrefixSearchTermFinder.
-Qed.
-Print foo13.
-
-Lemma foo12 :
-  forall l l' : name,
-    ?[IsPrefix_dec l l'] = false ->
-    ?[list_eq_dec string_dec l l'] = false.
-Proof.
-  intros; find_if_inside; subst.
-  [ rewrite <- prefix_reflexive in H | ]; auto.
-Qed.
-
-Lemma foo11 {heading}
-: forall l,
-    map (ilist_hd (As:=cons heading nil ))
-        (Build_single_Tuple_list l) = l.
-Proof.
-  induction l; simpl; congruence.
-Qed. *)
-
-    Lemma refine_filtered_list {A}
-    : forall (xs : list A)
-             (P : Ensemble A)
-             (P_dec : DecideableEnsemble P),
-        refine (filtered_list xs P)
-               (ret (filter dec xs)).
-    Proof.
-      unfold filtered_list; induction xs; intros.
-      - reflexivity.
-      - simpl; setoid_rewrite IHxs.
-        simplify with monad laws.
-        destruct (dec a) eqn: eq_dec_a;
-          [ setoid_rewrite dec_decides_P in eq_dec_a; refine pick val true |
-            setoid_rewrite Decides_false in eq_dec_a; refine pick val false ];
-          auto; simplify with monad laws; reflexivity.
-    Qed.
-
-    Definition find_upperbound {A} (f : A -> nat) (ns : list A) : list A :=
-      let max := fold_right
-                   (fun n acc => max (f n) acc) O ns in
-      filter (fun n => NPeano.leb max (f n)) ns.
-
-    Lemma fold_right_max_is_max {A}
-    : forall (f : A -> nat) ns n,
-        List.In n ns -> f n <= fold_right (fun n acc => max (f n) acc) 0 ns.
-    Proof.
-      induction ns; intros; inversion H; subst; simpl;
-      apply NPeano.Nat.max_le_iff; [ left | right ]; auto.
-    Qed.
-
-    Lemma fold_right_higher_is_higher {A}
-    : forall (f : A -> nat) ns x,
-        (forall r, List.In r ns -> f r <= x) ->
-        fold_right (fun n acc => max (f n) acc) 0 ns <= x.
-    Proof.
-      induction ns; simpl; intros; [ apply le_0_n | ].
-      apply NPeano.Nat.max_lub.
-      apply H; left; auto.
-      apply IHns; intros; apply H; right; auto.
-    Qed.
-
-    Lemma find_upperbound_highest_length {A}
-    : forall (f : A -> nat) ns n,
-        List.In n (find_upperbound f ns) -> forall n', List.In n' ns -> (f n) >= (f n').
-    Proof.
-      unfold ge, find_upperbound; intros.
-      apply filter_In in H; destruct H; apply NPeano.leb_le in H1.
-      rewrite <- H1; clear H1 H n.
-      apply fold_right_max_is_max; auto.
-    Qed.
-
-    (* Lemma find_upperbound_upperbound {A}
-    : forall (f : A -> nat) ns n, List.In n (find_upperbound f ns) <->
-                                    List.In n ns /\ upperbound f ns n.
-    Proof.
-      unfold upperbound, ge; intros; split; intros; try split.
-      - unfold find_upperbound in H; apply filter_List.In in H; tauto.
-      - apply find_upperbound_highest_length; auto.
-      - destruct H; unfold find_upperbound.
-        apply filter_List.In; split; try assumption.
-        apply NPeano.leb_le.
-        pose proof (fold_right_max_is_max f _ _ H).
-        pose proof (fold_right_higher_is_higher f _ H0).
-        auto.
-    Qed. *)
-
-    Instance DecideableEnsembleUpperbound {A} (f : A -> nat) ns :
-      DecideableEnsemble (upperbound f ns) :=
-      {| dec n := NPeano.leb (fold_right (fun n acc => max (f n) acc) O ns) (f n) |}.
-    Proof.
-      unfold upperbound, ge; intros; rewrite NPeano.leb_le; intuition.
-      - remember (f a); clear Heqn; subst; eapply le_trans;
-        [ apply fold_right_max_is_max; apply H0 | assumption ].
-      - eapply fold_right_higher_is_higher; eauto.
-    Defined.
-
-    Corollary refine_find_upperbound {A}
-    : forall (f : A -> nat) ns,
-        refine ([[n in ns | upperbound f ns n]])
-               (ret (find_upperbound f ns)).
-    Proof.
-      intros.
-      setoid_rewrite refine_filtered_list with (P_dec := DecideableEnsembleUpperbound f ns).
-      reflexivity.
-    Qed.
-
-    Lemma foo16 :
-      forall ns s,
-        (forall n', List.In n' ns -> IsPrefix (get_name n') s)
-        -> forall n n', List.In n (find_upperbound name_length ns)
-                        -> List.In n' (find_upperbound name_length ns)
-                        -> get_name n = get_name n'.
-    Proof.
-      unfold find_upperbound, name_length; intros ns s H0 n n' H H1.
-      apply filter_In in H; destruct H; apply filter_In in H1; destruct H1.
-      pose proof (H0 _ H); pose proof (H0 _ H1).
-      apply NPeano.leb_le in H2; apply NPeano.leb_le in H3.
-      pose proof (fold_right_max_is_max name_length ns n H) as H2'.
-      pose proof (fold_right_max_is_max name_length ns n' H1) as H3'.
-      unfold name_length in *.
-      apply (le_antisym _ _ H2') in H2; apply (le_antisym _ _ H3') in H3.
-      rewrite <- H2 in H3.
-      unfold IsPrefix in *; destruct H4; destruct H5; rewrite <- H5 in H4.
-      clear H2' H3' H H2 H0 H1 H5 s ns.
-      remember (get_name n); remember (get_name n'); clear Heql Heql0.
-      revert x0 l l0 H4 H3.
-      induction x; destruct x0; intros.
-      - repeat rewrite app_nil_r in H4; assumption.
-      - apply f_equal with (f := @Datatypes.length string) in H4.
-        repeat rewrite app_length in H4; subst; exfalso; simpl in *; omega.
-      - apply f_equal with (f := @Datatypes.length string) in H4.
-        repeat rewrite app_length in H4; subst; exfalso; simpl in *; omega.
-      - rewrite app_comm_cons' with (As := l) in H4.
-        rewrite app_comm_cons' with (As := l0) in H4.
-        apply IHx in H4; [ apply app_inj_tail in H4; destruct H4; auto |
-        repeat rewrite app_length; rewrite H3; reflexivity ].
-    Qed.
-
-    Ltac find_if_inside_eqn :=
-      match goal with
-        | [ |- context[if ?X then _ else _] ] => destruct X eqn: ?
-        | [ H : context[if ?X then _ else _] |- _ ]=> destruct X eqn: ?
-      end.
-
-    (* Implement the check for an exact match *)
-    Lemma foo19
-    : forall ns s,
-        (forall n', List.In n' ns -> IsPrefix (get_name n') s) ->
-        refine {b : bool |
-                decides b
-                        (~
-                           (exists x : DNSRRecord,
-                              List.In x (find_upperbound name_length ns) /\ s <> (get_name x)))}
-               (ret match find_upperbound name_length ns with
-                      | nil => true
-                      | n' :: _ => ?[s == (get_name n')]
-                    end).
-    Proof.
-      computes_to_econstructor; simpl in H; intros; computes_to_inv.
-      subst; unfold decides; pose proof (foo16 ns H); clear H.
-      remember (find_upperbound name_length ns) as l.
-      unfold If_Then_Else.
-      find_if_inside_eqn.
-      - unfold not; intros; repeat destruct H; apply H1; clear H1; destruct l;
-        [ inversion H | subst; apply H0 with (n := d) in H ];
-        [ find_if_inside; [ subst; auto | inversion Heqb ] | simpl; left; auto ].
-      - unfold not; intros; apply H; clear H; destruct l; try inversion Heqb.
-        exists d; split; [ simpl; left; auto | intros; rewrite <- H in Heqb ].
-        find_if_inside; [ discriminate | unfold not in *; apply n; auto ].
-    Qed.
-
-    Lemma in_list_exists {A}
-    : forall (xs : list A) x, List.In x xs -> exists n, nth_error xs n = Some x.
-    Proof.
-      intros; induction xs; inversion H; subst.
-      exists 0; reflexivity.
-      apply IHxs in H0; destruct_ex; exists (1 + x0); auto.
-    Qed.
-
-    Lemma in_list_preserve_filter {A}
-    : forall (f : A -> bool) xs x, List.In x (filter f xs) -> List.In x xs.
-    Proof.
-      intros; apply (filter_In f x xs) in H; tauto.
-    Qed.
-
-    Lemma foo20
-    : forall ns n s
-             (HH : forall t t' n n', n <> n'
-                                     -> nth_error ns n =  Some t
-                                     -> nth_error ns n' = Some t'
-                                     -> get_name t = get_name t'
-                                     -> t!sTYPE <> CNAME),
-        (forall n', List.In n' ns -> IsPrefix (get_name n') s) ->
-        refine {b' |
-                forall b : Tuple,
-                  b' = Some b <->
-                  List.In b (find_upperbound name_length ns) /\
-                  b!sTYPE = CNAME /\ n <> CNAME}
-               (ret match (find_upperbound name_length ns) with
-                      | nil => None
-                      | n' :: _ => if CNAME == (n'!sTYPE)
-                                   then if n == CNAME
-                                        then None
-                                        else Some n'
-                                   else None
-                    end).
-    Proof.
-      unfold refine, not; intros; pose proof (foo16 ns H); clear H.
-      remember (find_upperbound name_length ns) as l.
-      computes_to_inv; computes_to_econstructor; split; intros.
-      - destruct l; [ subst; inversion H | ].
-        repeat find_if_inside_eqn; subst; try inversion H; subst.
-        repeat split; [ simpl; left | symmetry | ]; auto.
-      - destruct H as [? [? ?] ]; destruct l; [ inversion H | subst ].
-        inversion H; unfold not in *.
-        + repeat find_if_inside; subst; auto; exfalso; auto.
-        + assert (d = b).
-          * pose proof (in_eq d l).
-            pose proof H; rewrite Heql in H5; pose proof (in_list_preserve_filter _ ns b H5); clear H5.
-            pose proof H4; rewrite Heql in H5; pose proof (in_list_preserve_filter _ ns d H5); clear H5.
-            pose proof (in_list_exists ns b H6); pose proof (in_list_exists ns d H7); destruct_ex; pose proof (H1 d b H4 H).
-            destruct (beq_nat x0 x) eqn: eq; [ rewrite beq_nat_true_iff in eq; subst; rewrite H8 in H5; inversion H5; auto | ].
-            rewrite beq_nat_false_iff in eq; symmetry in H9.
-            pose proof (HH b d x0 x eq H5 H8 H9); exfalso; auto.
-          * repeat find_if_inside; subst; [ exfalso; apply H3 | | exfalso; apply n0 ]; auto.
-    Qed.
-
-    Lemma refine_If_Opt_Then_Else_ret {A B} :
-      forall i (t : A -> B) (e : B),
-        refine (@If_Opt_Then_Else A (Comp B) i (fun a => ret (t a)) (ret e))
-               (ret (@If_Opt_Then_Else A B i t e)).
-    Proof.
-      destruct i; reflexivity.
-    Qed.
-
-Lemma refine_decides_forall_In' :
-  forall {A} l (P: A -> Prop) (P_Dec : DecideableEnsemble P),
-    refine {b | decides b (forall (x: A), List.In x l -> P x)}
-           {b | decides b (~ exists (x : A), List.In x l /\ ~ P x)}.
-Proof.
-  unfold refine; intros; computes_to_inv.
-  computes_to_constructor.
-  destruct v; simpl in *; intros.
-  case_eq (dec x); intros; try rewrite <- (dec_decides_P); eauto.
-  elimtype False; eapply H; eexists; intuition eauto.
-  rewrite <- dec_decides_P in H2; congruence.
-  unfold not in *; intros.
-  eapply H; intros.
-  destruct H1; intuition.
-Qed.
-
-Transparent FueledFix.
-Opaque Query_For.
+Print MostlySharpened.
 
 Theorem DnsManual :
   MostlySharpened DnsSpec.
 Proof.
-
-  start honing QueryStructure.
+  (* unfold MostlySharpened. *)
+  start honing QueryStructure. (* what does this do? what's the stuff in the context? *)
 
   (* Implement the constraint checks as queries. *)
-  hone method "AddData".
-  { subst_all.
+  (* original: update "AddData" (t : DNSRRecord) : bool :=
+      Insert t into sCOLLECTIONS *)
+  (* mutates, so need to check constraints on NAME/CNAME *)
+  hone method "AddData".        (* ? *)
+  {
+    (* AddData has been expanded in method StringId0 *)
+    (* refine (AddData body) (H r_n n) <-- what is that? *)
+    (* H := existential variable of the correct (?) type,
+       r_n : UnConstrQueryStructure DnsSchema, n : DNSRRecord*)
+    (* x1 = check constraint between n (the record) and every other tuple  *)
+    (* x2 = check constraint between every other tuple and n (the record) *)
+    (* doesn't know that the constraint is symmetric? *)
+
+    (* one-liner with rewrites? *)
+    subst_all.
     match goal with
       |- refine _ (?H _ _) => let id := fresh in set (id := H) in *
-    end.
-    setoid_rewrite foo3.
-    setoid_rewrite foo5.
+    end.                        (* replace ex var with name H again *)
+    setoid_rewrite refine_count_constraint_broken.        (* refine x1 *)
+    setoid_rewrite refine_count_constraint_broken'.        (* refine x2 *)
+    Check refine_If_Then_Else_Bind.
+    Check Bind_refine_If_Then_Else.
     setoid_rewrite refine_If_Then_Else_Bind.
     setoid_rewrite Bind_refine_If_Then_Else.
     etransitivity.
+    Check refine_If_Then_Else.
     apply refine_If_Then_Else.
     - simplify with monad laws.
-      apply refine_under_bind; intros.
+      apply refine_under_bind; intros. (* x0 disappears? *)
+      Check refine_Count.
       setoid_rewrite refine_Count; simplify with monad laws.
       apply refine_under_bind; intros.
       (* remove duplicate check *)
-      setoid_rewrite foo7; eauto.
+      (* (simplifies x1) *)
+      setoid_rewrite refine_subcheck_to_filter; eauto.
       simplify with monad laws.
-      rewrite foo8 by apply foo9.
-      higher_order_1_reflexivity.
+      rewrite clear_nested_if by apply filter_nil_is_nil.
+      (* removes one of the repeated rets, and the filter dec -- how? *)
+      higher_order_1_reflexivity. (* ? where did the next goal come from? *)
       eauto with typeclass_instances.
     - simplify with monad laws.
-      reflexivity.
-    - finish honing.
+      reflexivity.              (* refine (code) (existential variable) is cleared by reflexivity *)
+    - finish honing.            (* can finish honing anywhere? *)
   }
+  (* higher level of reasoning *)
 
   GenerateIndexesForAll
   ltac:(CombineCase2 matchFindSuffixIndex matchEqIndex)
@@ -839,6 +235,7 @@ Proof.
     finish honing.
    }
 
+  (* why stop honing AddData, hone Init, then come back to this? *)
     (* hone method "AddData". *) {
     etransitivity.
     setoid_rewrite refine_If_Then_Else_Bind.
@@ -908,7 +305,8 @@ Proof.
     simplify with monad laws.
     etransitivity.
     { apply refine_bind;
-      [ apply foo19; clear H2 H0;  admit | intro; higher_order_reflexivity ].
+      (* apply refine_check_one_longest_prefix_s. clear H2 H0. (* follows from the semantics of bagfind *) *)
+      [ apply refine_check_one_longest_prefix_s; clear H2 H0;  admit | intro; higher_order_reflexivity ].
     }
     simplify with monad laws.
     setoid_rewrite refine_if_If.
@@ -918,9 +316,12 @@ Proof.
     simplify with monad laws.
     etransitivity.
     { apply refine_bind;
-      [ eapply foo20; clear H2 H0 | intro; higher_order_reflexivity ].
-      intros; admit.
-      instantiate (1 := qname (questions d)); admit.
+      [ eapply refine_check_one_longest_prefix_CNAME; clear H2 H0 | intro; higher_order_reflexivity ].
+      intros. admit.            (* result of data integrity constraints *)
+      (* should prove it earlier? already dropped the proof *)
+      (* drop condition before honing? *)
+      instantiate (1 := qname (questions d)). admit.
+    (* same as 1st admit? *)
     }
     simplify with monad laws.
     apply refine_If_Opt_Then_Else_Bind.
