src/Examples/DnsServer/DnsLemmas.v
@@ -1,0 +1,712 @@
+Require Import Coq.Vectors.Vector
+        Coq.Strings.Ascii
+        Coq.Bool.Bool
+        Coq.Bool.Bvector
+        Coq.Lists.List.
+
+Require Import Fiat.QueryStructure.Automation.AutoDB
+        Fiat.QueryStructure.Implementation.DataStructures.BagADT.BagADT
+        Fiat.Examples.DnsServer.packet
+        Fiat.QueryStructure.Automation.IndexSelection
+        Fiat.QueryStructure.Specification.SearchTerms.ListPrefix
+        Fiat.QueryStructure.Automation.SearchTerms.FindSuffixSearchTerms
+        Fiat.QueryStructure.Automation.QSImplementation.
+
+
+Open Scope list.
+
+Definition upperbound {A} (f : A -> nat) (rs : list A) (r : A) :=
+  forall r', List.In r' rs -> f r >= f r'.
+
+Section FueledFix.
+  (* TODO: Find a home for these more definitions in the Common folder. *)
+
+  Variable A : Type. (* Argument Type *)
+  Variable R : Type. (* Return Type *)
+
+  Fixpoint FueledFix (fuel : nat) (base : Comp R)
+                     (body : (A -> Comp R) -> A -> Comp R) (arg : A)
+  : Comp R :=
+    match fuel with
+      | O => base
+      | S fuel' => body (FueledFix fuel' base body) arg
+    end.
+End FueledFix.
+
+(* Can rewrite under Fueled Fix at the moment,
+as the condition on the body is not a proper relation. :p *)
+(* TODO: figure out a definition for pointwise_refine that is a
+   proper (i.e. reflexive and transitive) relation.
+ *)
+(*
+Print respectful.
+
+Definition pointwise_refine {A R}
+  (f g : (A -> Comp R) -> A -> Comp R) :=
+  forall (rec rec' : A -> Comp R) (a : A),
+    pointwise_relation A (@refine R) rec rec'
+    -> refine (f rec a) (g rec' a).
+
+Lemma reflexive_pR {A R : Type} :
+  forall A R, Reflexive (@pointwise_refine A R).
+Proof.
+  unfold Reflexive, pointwise_refine, pointwise_relation.
+  intros.
+  (* Doesn't work if x is (fun rec a => {r | ~ rec ~> r} :p *)
+Admitted.
+
+Lemma transitive_pR {A R : Type} :
+  forall A R, Transitive (@pointwise_refine A R).
+Proof.
+  unfold Transitive, pointwise_refine, pointwise_relation; intros.
+  etransitivity.
+  apply H; eauto.
+  apply H0. reflexivity.
+Qed.
+
+Add Parametric Morphism A R i
+: (@FueledFix A R i)
+    with signature
+    ((@refine R)
+       ==> (@pointwise_refine A R)
+      ==> (@eq A)
+      ==> (@refine R))
+      as refineFix.
+Proof.
+  simpl; induction i; intros; simpl.
+  - assumption.
+  - unfold pointwise_refine, pointwise_relation, Proper, respectful in *.
+    eapply H0.
+    intros.
+    generalize (IHi _ _ H _ _ H0 a); eauto.
+Qed.
+*)
+
+(* TODO: Agree on a notation for our fueled fix function. *)
+Notation "'Repeat' fuel 'initializing' a 'with' arg 'defaulting' rec 'with' base {{ bod }} " :=
+  (FueledFix fuel base (fun rec a => bod) arg)
+    (no associativity, at level 50,
+     format "'Repeat' '[hv'  fuel  '/' 'initializing'  a  'with'  arg '/'  'defaulting'  rec  'with'  base  '/' {{ bod  }} ']' ").
+
+Section FueledFixRefinements.
+  (* TODO: Find a home for these refinements in the Computation folder. *)
+
+  Variable A : Type. (* Argument Type *)
+  Variable R : Type. (* Return Type *)
+
+  (* TODO Lemmas for refining FueledFix. *)
+
+  Lemma refine_FueledFix_Bind (B : Type) :
+    forall fuel body (base : Comp R) (arg : A) (k k' : R -> Comp B),
+      refine (r <- base; k r) (r <- base; k' r)
+      -> (forall fuel',
+            refine (a <- FueledFix fuel' base body arg; k a)
+                   (a <- FueledFix fuel' base body arg; k' a)
+            -> refine
+                 (a <- FueledFix (S fuel') base body arg; k a)
+                 (a <- FueledFix (S fuel') base body arg; k' a))
+      ->  refine (a <- FueledFix fuel base body arg; k a)
+                 (a <- FueledFix fuel base body arg; k' a).
+  Proof.
+    induction fuel; eauto.
+  Qed.
+
+End FueledFixRefinements.
+
+Section FilteredList.
+
+  Definition filtered_list {A}
+             (xs : list A)
+             (P : Ensemble A)
+    := fold_right (fun (a : A) (l : Comp (list A)) =>
+                     l' <- l;
+                     b <- { b | decides b (P a) };
+                     if b
+                     then ret (a :: l')
+                     else ret l'
+                  ) (ret nil) xs.
+
+End FilteredList.
+
+(* Agree on this notation. *)
+Notation "'unique' b , P ->> s 'otherwise' ->> s'" :=
+  (b' <- {b' | forall b, b' = Some b <-> P};
+   If_Opt_Then_Else b' (fun b => s) s') (at level 70).
+
+Definition is_empty {A} (l : list A) :=
+  match l with nil => true | _ => false end.
+
+Definition get_name (r : DNSRRecord) : list string := r!sNAME.
+Definition name_length (r : DNSRRecord) := List.length (get_name r).
+
+Notation "[[ x 'in' xs | P ]]" := (filtered_list xs (fun x => P)) (at level 70) : comp_scope.
+
+(* -------------------------------------------------------------------------------------- *)
+
+(* Refinement lemmas *)
+
+(* First, lemmas that help with honing the AddData method in DnsManual. They're related to implementing the data constraint (on DnsSchema) as a query. *)
+
+(* if the record's type isn't CNAME, there's no need to check against the other records;
+it's independent of the other records *)
+Lemma refine_not_CNAME__independent :
+  forall (n : DNSRRecord) (R : @IndexedEnsemble DNSRRecord),
+    n!sTYPE <> CNAME
+    -> refine {b |
+               decides b
+                       (forall tup' : IndexedTuple,
+                          R tup' ->
+                          n!sNAME = (indexedElement tup')!sNAME -> n!sTYPE <> CNAME)}
+
+              (ret true).
+Proof.
+  (* where are pick and val from? *)
+  intros; refine pick val true; [ reflexivity | simpl; intros; assumption ].
+Qed.
+
+(* if the record's type *is* CNAME, then refine the forall check against other records into 
+an existential (exists a record with the same name), and return the opposite *)
+Lemma refine_is_CNAME__forall_to_exists :
+  forall (n : DNSRRecord) (R : @IndexedEnsemble DNSRRecord),
+    n!sTYPE = CNAME
+    -> refine {b |
+               decides b
+                       (forall tup' : IndexedTuple,
+                          R tup' ->
+                          n!sNAME = (indexedElement tup')!sNAME -> n!sTYPE <> CNAME)}
+              (b <- {b |
+                     decides b
+                             (exists tup' : IndexedTuple,
+                                R tup' /\
+                                n!sNAME = (indexedElement tup')!sNAME)};
+               ret (negb b)).
+Proof.
+   repeat match goal with
+    | _ : _ ↝ _ |- _ => computes_to_inv
+    | _ : negb ?v = _ |- _ => destruct v; simpl in *; subst
+    | _ : ex _ |- _ => destruct_ex
+    | _ => progress first [ intro | computes_to_econstructor | simpl; intuition; eauto ]
+          end.
+Qed.
+
+(* very similar to refine_is_CNAME__forall_to_exists; 
+they start with the same set, but refine_forall_to_exists refines it with an extra end condition. changes the (forall x, ~P x) check into (exists x, P x) and returns !x, adding the condition in the forall *)
+Lemma refine_forall_to_exists :
+  forall (n : DNSRRecord) (R : @IndexedEnsemble DNSRRecord),
+    refine {b |
+            decides b
+                    (forall tup' : IndexedTuple,
+                       R tup' ->
+                       (indexedElement tup')!sNAME = n!sNAME
+                       -> (indexedElement tup')!sTYPE <> CNAME)}
+           (b <- {b |
+                  decides b
+                          (exists tup' : IndexedTuple,
+                             R tup' /\
+                             n!sNAME = (indexedElement tup')!sNAME
+                             /\ (indexedElement tup')!sTYPE = CNAME)};
+            ret (negb b)).
+Proof.                          (* same proof as refine_is_CNAME__forall_to_exists *)
+  repeat match goal with
+    | _ : _ ↝ _ |- _ => computes_to_inv
+    | _ : negb ?v = _ |- _ => destruct v; simpl in *; subst
+    | _ : ex _ |- _ => destruct_ex
+    | _ => progress first [ intro | computes_to_econstructor | simpl; intuition; eauto ]
+         end.
+Qed.
+
+(* in AddData, simplifies x1 from large For/Where/Return expression to [ret (filter dec a0)] *)
+
+(* refine a check into a filter, given the results of a sub-check 
+uses P' decision procedure invisibly in DecideableEnsembles.dec by the magic of typeclasses
+(try Set Printing Implicit) *)
+Lemma refine_subcheck_to_filter {heading}
+: forall (R : Ensemble (@IndexedTuple heading))
+         (P : Ensemble Tuple) (P_dec : DecideableEnsemble P)
+         (l : list Tuple),
+    For (QueryResultComp
+           R
+           (fun tup => Where (P tup) (* tuple is in P *)
+                             (Return tup))) ↝ l  ->
+    forall (P' : Ensemble Tuple) (P'_dec : DecideableEnsemble P'),
+      refine
+        (* assumption: subexpression with only [P tup] computes to l *)
+        (* note: P, P' are sets of tuples *)
+        (For (QueryResultComp
+                R
+                (fun tup => Where (P tup /\ P' tup)
+                                  (Return tup))))
+        (ret (filter DecideableEnsembles.dec l)).
+Proof.
+  Local Transparent Query_For.
+  unfold Query_For, QueryResultComp, Query_Return;
+    intros; computes_to_inv.
+  refine pick val _; eauto.
+  simplify with monad laws.
+  unfold refine; intros; computes_to_inv; computes_to_econstructor.
+  instantiate (1 := (filter (@dec _ _ P'_dec) v)).
+  - clear H0 H H' v1; generalize dependent v; induction v0.
+    + simpl; intros; computes_to_inv; subst; reflexivity.
+    + simpl; intros; computes_to_inv; subst; apply IHv0 in H'0'; clear IHv0.
+      destruct (@dec _ P' P'_dec a) eqn: dec_a; unfold Query_Where in *; destruct H'0.
+      * pose proof dec_a as dec_a'; apply dec_decides_P in dec_a.
+        repeat computes_to_inv; repeat computes_to_econstructor.
+        intuition eauto. eauto.
+        apply eq_ret_compute; destruct (@dec _ P P_dec a) eqn: dec__a.
+        apply dec_decides_P in dec__a; apply H in dec__a;
+        computes_to_inv; subst; simpl; rewrite dec_a'; reflexivity.
+        apply Decides_false in dec__a; apply H0 in dec__a; subst; reflexivity.
+      * pose proof dec_a as dec_a'; apply Decides_false in dec_a.
+        repeat computes_to_inv; repeat computes_to_econstructor.
+        intuition eauto. eauto.
+        apply eq_ret_compute; destruct (@dec _ P P_dec a) eqn: dec__a.
+        apply dec_decides_P in dec__a; apply H in dec__a;
+        computes_to_inv; subst; simpl; rewrite dec_a'; reflexivity.
+        apply Decides_false in dec__a; apply H0 in dec__a; subst; reflexivity.
+  - refine pick val _; auto; subst.
+    apply filter_permutation_morphism; [ reflexivity | assumption ].
+Qed.
+
+(* clear_nested_if, using filter_nil_is_nil, clear the nested if/then in honing AddData *)
+Lemma clear_nested_if {A}
+: forall (c c' : bool) (t e e' : A),
+    (c = true -> c' = true)
+    -> (if c then (if c' then t else e) else e') = if c then t else e'.
+Proof.
+  intros; destruct c; destruct c'; try reflexivity.
+  assert (true = true); [ reflexivity | apply H in H0; discriminate ].
+Qed.
+
+(* if a list is empty, the result of filtering the list with anything will still be empty *)
+Lemma filter_nil_is_nil {A}
+: forall (l : list A) (pred : A -> bool),
+    beq_nat (Datatypes.length l) 0 = true
+    ->  beq_nat (Datatypes.length (filter pred l)) 0 = true.
+Proof.
+  induction l; intros; simpl; try inversion H.
+  reflexivity.
+Qed.
+
+Lemma andb_implication_preserve :
+  forall a b, (a = true -> b = true) -> a = b && a.
+Proof.
+  intros; destruct a; destruct b; symmetry; auto.
+Qed.
+Lemma andb_permute :
+  forall a b c, a && (b && c) = b && (a && c).
+  intros.
+  repeat rewrite andb_assoc.
+  replace (a && b) with (b && a) by apply andb_comm.
+  reflexivity.
+Qed.
+
+(*Ltac PrefixSearchTermFinderEqSolve :=
+  intros; unfold PrefixSearchTermMatcher; simpl;
+   apply andb_implication_preserve; find_if_inside; intros;
+   match goal with
+     | H : _ = _ |- _ =>
+       setoid_rewrite H;
+         erewrite prefixBool_reflexive; reflexivity
+     | _ => erewrite prefixBool_reflexive; reflexivity
+     | _ => discriminate
+   end.
+Ltac PrefixSearchTermNormalizer idx :=
+  generalize dependent idx;
+  let a' := fresh in
+  let ha := fresh in
+  match goal with
+    | |- forall a, _ = PrefixSearchTermMatcher ?st (@?h a) =>
+      intros a'; remember (h a') as ha; generalize ha
+  end.
+Ltac PrefixSearchTermFinder' idx :=
+  PrefixSearchTermNormalizer idx;
+  match goal with
+    (* case prefix match *)
+    | |- forall a, prefixBool ?n a!sNAME && @?f a = PrefixSearchTermMatcher ?st a =>
+      instantiate (1 := {| pst_name := n; pst_filter := f |}); reflexivity
+    (* case equality *)
+    | |- forall a, ?[list_eq_dec string_dec ?n a!sNAME] && @?f a =
+                   PrefixSearchTermMatcher ?st a =>
+      instantiate
+        (1 := {| pst_name := n;
+                 pst_filter := fun a => ?[list_eq_dec string_dec n a!sNAME] && f a |});
+        PrefixSearchTermFinderEqSolve
+    | |- forall a, ?[list_eq_dec string_dec a!sNAME ?n] && @?f a =
+                   PrefixSearchTermMatcher ?st a =>
+      instantiate
+        (1 := {| pst_name := n;
+                 pst_filter := fun a => ?[list_eq_dec string_dec a!sNAME n] && f a |});
+        PrefixSearchTermFinderEqSolve
+  end.
+Ltac AdjustAndRec terminal term :=
+  let aterm := fresh in
+  first [
+      (* if we get the exact match, we're done !*)
+      assert (aterm : terminal = term) by reflexivity; clear aterm |
+      match term with
+        | ?left && ?right =>
+          first [
+              (* if the left term is the exact match, also done! *)
+              assert (aterm : left = terminal) by reflexivity; clear aterm |
+              (* if the right term is the exact match, just need to switch! *)
+              assert (aterm : right = terminal) by reflexivity; clear aterm;
+                replace (left && right) with
+                (right && left) by apply andb_comm |
+              (* now try recursively on the left term *)
+              (AdjustAndRec terminal left);
+                match goal with
+                  | |- context [ (terminal && ?rem) && right ] =>
+                    replace ((terminal && rem) && right) with
+                    (terminal && (rem && right)) by apply andb_assoc
+                end |
+              (* and now the righ term *)
+              (AdjustAndRec terminal right);
+                match goal with
+                  | |- context [ left && (terminal && ?rem) ] =>
+                    replace (left && (terminal && rem)) with
+                    (terminal && (left && rem)) by apply andb_permute
+                end ]
+      end ].
+Ltac AdjustAnd terminal ensure_and :=
+  match goal with
+    | |- ?filter = _ => AdjustAndRec terminal filter
+  end;
+  match ensure_and with
+    | true =>
+      match goal with
+        | |- _ && _ = _ => idtac
+        | |- ?x = _ => rewrite <- (andb_true_r x)
+      end
+    | false => idtac
+  end.
+Ltac PrefixSearchTermFinder :=
+  let idx := fresh in
+  intros idx;
+  match goal with
+    | |- context [ prefixBool ?n ?n' ] =>
+      AdjustAnd (prefixBool n n') true; PrefixSearchTermFinder' idx
+    (* ensure_and can be false, but need some more thought *)
+    | |- context [ ?[list_eq_dec string_dec ?n ?n'] ] =>
+      AdjustAnd (?[list_eq_dec string_dec n n']) true; PrefixSearchTermFinder' idx
+    | |- _ => PrefixSearchTermNormalizer idx;
+        match goal with
+          (* catch all case; ignore search term, use only the filter *)
+          (* only when wildcard is idtac, when this tactic gets used *)
+          | |- forall a, @?f a = PrefixSearchTermMatcher ?st a =>
+            instantiate (1 := {| pst_name := nil; pst_filter := f |}); reflexivity
+        end
+  end.
+
+Lemma foo10
+: forall (n : DNSRRecord) (b c d e : bool), exists st, forall (a : DNSRRecord * nat),
+    ?[list_eq_dec string_dec (fst a)!sNAME n!sNAME] =
+    PrefixSearchTermMatcher st (fst a).
+Proof.
+  eexists.
+  PrefixSearchTermFinder.
+Qed.
+Print foo10.
+Lemma foo10' : forall n : DNSRRecord, forall b c d, exists st, forall (a : DNSRRecord * nat),
+    b && ( c && d ) && (?[list_eq_dec string_dec (fst a)!sNAME n!sNAME]) && (?[RRecordType_dec (fst a)!sTYPE CNAME]) =
+    PrefixSearchTermMatcher st (fst a).
+Proof.
+  eexists; PrefixSearchTermFinder.
+Qed.
+Print foo10'.
+Lemma foo13
+: forall n : DNSRRecord, exists st, forall a : DNSRRecord,
+    prefixBool (n!sNAME) (a!sNAME)  =
+    PrefixSearchTermMatcher st a.
+Proof.
+  eexists; PrefixSearchTermFinder.
+Qed.
+Print foo13.
+
+Lemma foo12 :
+  forall l l' : name,
+    ?[IsPrefix_dec l l'] = false ->
+    ?[list_eq_dec string_dec l l'] = false.
+Proof.
+  intros; find_if_inside; subst.
+  [ rewrite <- prefix_reflexive in H | ]; auto.
+Qed.
+
+Lemma foo11 {heading}
+: forall l,
+    map (ilist_hd (As:=cons heading nil ))
+        (Build_single_Tuple_list l) = l.
+Proof.
+  induction l; simpl; congruence.
+Qed. *)
+
+    Lemma refine_filtered_list {A}
+    : forall (xs : list A)
+             (P : Ensemble A)
+             (P_dec : DecideableEnsemble P),
+        refine (filtered_list xs P)
+               (ret (filter dec xs)).
+    Proof.
+      unfold filtered_list; induction xs; intros.
+      - reflexivity.
+      - simpl; setoid_rewrite IHxs.
+        simplify with monad laws.
+        destruct (dec a) eqn: eq_dec_a;
+          [ setoid_rewrite dec_decides_P in eq_dec_a; refine pick val true |
+            setoid_rewrite Decides_false in eq_dec_a; refine pick val false ];
+          auto; simplify with monad laws; reflexivity.
+    Qed.
+
+    Definition find_upperbound {A} (f : A -> nat) (ns : list A) : list A :=
+      let max := fold_right
+                   (fun n acc => max (f n) acc) O ns in
+      filter (fun n => NPeano.leb max (f n)) ns.
+
+    Lemma fold_right_max_is_max {A}
+    : forall (f : A -> nat) ns n,
+        List.In n ns -> f n <= fold_right (fun n acc => max (f n) acc) 0 ns.
+    Proof.
+      induction ns; intros; inversion H; subst; simpl;
+      apply NPeano.Nat.max_le_iff; [ left | right ]; auto.
+    Qed.
+
+    Lemma fold_right_higher_is_higher {A}
+    : forall (f : A -> nat) ns x,
+        (forall r, List.In r ns -> f r <= x) ->
+        fold_right (fun n acc => max (f n) acc) 0 ns <= x.
+    Proof.
+      induction ns; simpl; intros; [ apply le_0_n | ].
+      apply NPeano.Nat.max_lub.
+      apply H; left; auto.
+      apply IHns; intros; apply H; right; auto.
+    Qed.
+
+    Lemma find_upperbound_highest_length {A}
+    : forall (f : A -> nat) ns n,
+        List.In n (find_upperbound f ns) -> forall n', List.In n' ns -> (f n) >= (f n').
+    Proof.
+      unfold ge, find_upperbound; intros.
+      apply filter_In in H; destruct H; apply NPeano.leb_le in H1.
+      rewrite <- H1; clear H1 H n.
+      apply fold_right_max_is_max; auto.
+    Qed.
+
+    (* Lemma find_upperbound_upperbound {A}
+    : forall (f : A -> nat) ns n, List.In n (find_upperbound f ns) <->
+                                    List.In n ns /\ upperbound f ns n.
+    Proof.
+      unfold upperbound, ge; intros; split; intros; try split.
+      - unfold find_upperbound in H; apply filter_List.In in H; tauto.
+      - apply find_upperbound_highest_length; auto.
+      - destruct H; unfold find_upperbound.
+        apply filter_List.In; split; try assumption.
+        apply NPeano.leb_le.
+        pose proof (fold_right_max_is_max f _ _ H).
+        pose proof (fold_right_higher_is_higher f _ H0).
+        auto.
+    Qed. *)
+
+    Instance DecideableEnsembleUpperbound {A} (f : A -> nat) ns :
+      DecideableEnsemble (upperbound f ns) :=
+      {| dec n := NPeano.leb (fold_right (fun n acc => max (f n) acc) O ns) (f n) |}.
+    Proof.
+      unfold upperbound, ge; intros; rewrite NPeano.leb_le; intuition.
+      - remember (f a); clear Heqn; subst; eapply le_trans;
+        [ apply fold_right_max_is_max; apply H0 | assumption ].
+      - eapply fold_right_higher_is_higher; eauto.
+    Defined.
+
+    Corollary refine_find_upperbound {A}
+    : forall (f : A -> nat) ns,
+        refine ([[n in ns | upperbound f ns n]])
+               (ret (find_upperbound f ns)).
+    Proof.
+      intros.
+      setoid_rewrite refine_filtered_list with (P_dec := DecideableEnsembleUpperbound f ns).
+      reflexivity.
+    Qed.
+
+
+
+    (* used in refine_check_one_longest_prefix_s and refine_check_one_longest_prefix_CNAME *)
+    Lemma all_longest_prefixes_same :
+      forall (ns : list DNSRRecord) (s : list string),
+        (* the name (list string) of every record in the list is a prefix
+           of the given name (list string) *)
+        (* e.g. [com.google, com.google.us, com.google.us.scholar] with s = com.google.us.scholar *)
+        (forall (n' : DNSRRecord), List.In n' ns -> IsPrefix (get_name n') s)
+
+        (* for two records, if they both have the longest names in the list of records
+           (AND as before, they are prefixes of s)
+         then their names must be the same *)
+        -> forall n n' : DNSRRecord, List.In n (find_upperbound name_length ns)
+                        -> List.In n' (find_upperbound name_length ns)
+                        -> get_name n = get_name n'.
+    Proof.
+      unfold find_upperbound, name_length; intros ns s H0 n n' H H1.
+      apply filter_In in H; destruct H; apply filter_In in H1; destruct H1.
+      pose proof (H0 _ H); pose proof (H0 _ H1).
+      apply NPeano.leb_le in H2; apply NPeano.leb_le in H3.
+      pose proof (fold_right_max_is_max name_length ns n H) as H2'.
+      pose proof (fold_right_max_is_max name_length ns n' H1) as H3'.
+      unfold name_length in *.
+      apply (le_antisym _ _ H2') in H2; apply (le_antisym _ _ H3') in H3.
+      rewrite <- H2 in H3.
+      unfold IsPrefix in *; destruct H4; destruct H5; rewrite <- H5 in H4.
+      clear H2' H3' H H2 H0 H1 H5 s ns.
+      remember (get_name n); remember (get_name n'); clear Heql Heql0.
+      (* if 2 lists have the same length and are both prefixes of some list, they are the same list *)
+      revert x0 l l0 H4 H3.
+      induction x; destruct x0; intros.
+      - repeat rewrite app_nil_r in H4; assumption.
+      - apply f_equal with (f := @Datatypes.length string) in H4.
+        repeat rewrite app_length in H4; subst; exfalso; simpl in *; omega.
+      - apply f_equal with (f := @Datatypes.length string) in H4.
+        repeat rewrite app_length in H4; subst; exfalso; simpl in *; omega.
+      - rewrite app_comm_cons' with (As := l) in H4.
+        rewrite app_comm_cons' with (As := l0) in H4.
+        apply IHx in H4; [ apply app_inj_tail in H4; destruct H4; auto |
+        repeat rewrite app_length; rewrite H3; reflexivity ].
+    Qed.
+
+    Ltac find_if_inside_eqn :=
+      match goal with
+        | [ |- context[if ?X then _ else _] ] => destruct X eqn: ?
+        | [ H : context[if ?X then _ else _] |- _ ]=> destruct X eqn: ?
+      end.
+
+    (* ------------------ *)
+
+    (* These 3 lemmas relating to prefixes help hone the Process method in DnsManual *)
+
+    (* Implement the check for an exact match *)
+    (* uses all_longest_prefixes_same *)
+    Lemma refine_check_one_longest_prefix_s
+    : forall (ns : list DNSRRecord) (s : list string),
+        (* the name (list string) of every record in the list is a prefix
+           of the given name (list string) *)
+        (forall n' : DNSRRecord, List.In n' ns -> IsPrefix (get_name n') s) ->
+
+        (* there exists no record such that it is one of the longest prefixes of the name
+           AND is not the name itself -- refines to a computation that just checks the first
+           the name against the first longest prefix found. it's ok to just check the first
+           due to all_longest_prefixes_same: all longest prefixes must be the same *)
+        refine {b : bool |
+                decides b
+                        (~
+                           (exists x : DNSRRecord,
+                              List.In x (find_upperbound name_length ns) /\ s <> (get_name x)))}
+
+               (ret match find_upperbound name_length ns with
+                      | nil => true
+                      | n' :: _ => ?[s == (get_name n')]
+                    end).
+    Proof.
+      computes_to_econstructor; simpl in H; intros; computes_to_inv.
+      subst; unfold decides; pose proof (all_longest_prefixes_same ns H); clear H.
+      remember (find_upperbound name_length ns) as l.
+      unfold If_Then_Else.
+      find_if_inside_eqn.
+      - unfold not; intros; repeat destruct H; apply H1; clear H1; destruct l;
+        [ inversion H | subst; apply H0 with (n := d) in H ];
+        [ find_if_inside; [ subst; auto | inversion Heqb ] | simpl; left; auto ].
+      - unfold not; intros; apply H; clear H; destruct l; try inversion Heqb.
+        exists d; split; [ simpl; left; auto | intros; rewrite <- H in Heqb ].
+        find_if_inside; [ discriminate | unfold not in *; apply n; auto ].
+    Qed.
+
+    Lemma in_list_exists {A}
+    : forall (xs : list A) x, List.In x xs -> exists n, nth_error xs n = Some x.
+    Proof.
+      intros; induction xs; inversion H; subst.
+      exists 0; reflexivity.
+      apply IHxs in H0; destruct_ex; exists (1 + x0); auto.
+    Qed.
+
+    Lemma in_list_preserve_filter {A}
+    : forall (f : A -> bool) xs x, List.In x (filter f xs) -> List.In x xs.
+    Proof.
+      intros; apply (filter_In f x xs) in H; tauto.
+    Qed.
+
+    (* uses all_longest_prefixes_same; very similar to refine_check_one_longest_prefix_s but with an extra condition/Tuple type *)
+    Lemma refine_check_one_longest_prefix_CNAME
+    : forall (ns : list DNSRRecord) (n : RRecordType) (s : list string)
+             (HH : forall (t t' : DNSRRecord) (n n' : nat),
+                 n <> n'
+                 -> nth_error ns n  = Some t
+                 -> nth_error ns n' = Some t'
+                 -> get_name t      = get_name t'
+                 -> t!sTYPE <> CNAME),
+        (* forall HH? *)
+
+        (* as before, the name (list string) of every record in the list is a prefix
+           of the given name (list string) *)
+        (forall n' : DNSRRecord, List.In n' ns -> IsPrefix (get_name n') s) ->
+
+        (* Tuple type instead of record?
+        all "records" that contain the longest prefixes and are not CNAME, and n isn't CNAME  *)
+        (* this should be generalized to {b | List in ... /\ P} => match (...) with (P first one) *)
+        refine {b' : option Tuple |
+                forall b : Tuple,
+                  b' = Some b <->
+                  List.In b (find_upperbound name_length ns) /\
+                  b!sTYPE = CNAME /\ n <> CNAME}
+               (* refines to just checking the condition (with booleans) on the first longest prefix
+                using all_longest_prefixes_same *)
+               (ret match (find_upperbound name_length ns) with
+                      | nil => None
+                      | n' :: _ => if CNAME == (n'!sTYPE)
+                                   then if n == CNAME
+                                        then None
+                                        else Some n'
+                                   else None
+                    end).
+    Proof.
+      unfold refine, not; intros; pose proof (all_longest_prefixes_same ns H); clear H.
+      remember (find_upperbound name_length ns) as l.
+      computes_to_inv; computes_to_econstructor; split; intros.
+      - destruct l; [ subst; inversion H | ].
+        repeat find_if_inside_eqn; subst; try inversion H; subst.
+        repeat split; [ simpl; left | symmetry | ]; auto.
+      - destruct H as [? [? ?] ]; destruct l; [ inversion H | subst ].
+        inversion H; unfold not in *.
+        + repeat find_if_inside; subst; auto; exfalso; auto.
+        + assert (d = b).
+          * pose proof (in_eq d l).
+            pose proof H; rewrite Heql in H5; pose proof (in_list_preserve_filter _ ns b H5); clear H5.
+            pose proof H4; rewrite Heql in H5; pose proof (in_list_preserve_filter _ ns d H5); clear H5.
+            pose proof (in_list_exists ns b H6); pose proof (in_list_exists ns d H7); destruct_ex; pose proof (H1 d b H4 H).
+            destruct (beq_nat x0 x) eqn: eq; [ rewrite beq_nat_true_iff in eq; subst; rewrite H8 in H5; inversion H5; auto | ].
+            rewrite beq_nat_false_iff in eq; symmetry in H9.
+            (* HH instantiated here *)
+            pose proof (HH b d x0 x eq H5 H8 H9); exfalso; auto.
+          * repeat find_if_inside; subst; [ exfalso; apply H3 | | exfalso; apply n0 ]; auto.
+    Qed.
+
+    Lemma refine_If_Opt_Then_Else_ret {A B} :
+      forall i (t : A -> B) (e : B),
+        refine (@If_Opt_Then_Else A (Comp B) i (fun a => ret (t a)) (ret e))
+               (ret (@If_Opt_Then_Else A B i t e)).
+    Proof.
+      destruct i; reflexivity.
+    Qed.
+
+Lemma refine_decides_forall_In' :
+  forall {A} l (P: A -> Prop) (P_Dec : DecideableEnsemble P),
+    refine {b | decides b (forall (x: A), List.In x l -> P x)}
+           {b | decides b (~ exists (x : A), List.In x l /\ ~ P x)}.
+Proof.
+  unfold refine; intros; computes_to_inv.
+  computes_to_constructor.
+  destruct v; simpl in *; intros.
+  case_eq (dec x); intros; try rewrite <- (dec_decides_P); eauto.
+  elimtype False; eapply H; eexists; intuition eauto.
+  rewrite <- dec_decides_P in H2; congruence.
+  unfold not in *; intros.
+  eapply H; intros.
+  destruct H1; intuition.
+Qed.
+
+Transparent FueledFix.
+Opaque Query_For.
+
