src/Examples/DnsServer/DnsSchema.v
@@ -1,0 +1,16 @@
+Require Import
+        Fiat.QueryStructure.Automation.AutoDB
+        Fiat.Examples.DnsServer.packet.
+
+Definition DnsSchema :=
+  Query Structure Schema
+        [ relation sCOLLECTIONS has
+                   schema
+                  <sNAME :: name,
+                   sTYPE :: RRecordType,
+                   sCLASS :: RRecordClass,
+                   sTTL :: nat,
+                   sDATA :: string>
+          where (fun t t' => t!sNAME = t'!sNAME -> t!sTYPE <> CNAME) ]
+        (* constraint on every pair of tuples: an ip address cannot have multiple aliases? *)
+        enforcing [ ].
